still finishing casting proofs, changed type of nodes to nats for simplicity also think addressed bug where logic of list inclusion was wrong with choosing which connections should be considered inputs to the current edge state

src/GraphTranslation/BubbleSortTemp.v
@@ -239,73 +239,124 @@ Record zx_node := mk_node
   angle : R 
 }.
 
+Definition dummy_node := (mk_node 0%nat X_typ R0).
+(* 
 Definition eqb_zx_node (node1 node2 : zx_node) : bool :=
-  (id_no node1) =? (id_no node2).
+  (id_no node1) =? (id_no node2). *)
 
 Record zx_graph := mk_graph
-{ inputs : list zx_node;
-  outputs : list zx_node;
-  nodes : list zx_node;
-  edges : list (zx_node * zx_node)
+{ mapping : list zx_node;
+  inputs : list nat;
+  outputs : list nat;
+  nodes : list nat;
+  edges : list (nat * nat)
 }.
 
-Fixpoint inb_zx_node_list (l : list zx_node) (x : zx_node) : bool :=
+Definition get_zx_node_by_id (G : zx_graph) (n : nat) : zx_node :=
+  match (find (fun node => (id_no node) =? n) (mapping G)) with
+  | Some x => x
+  | _ => dummy_node (* Could change this*)
+  end
+.
+
+Definition inb_zx_node_list (l : list nat) (x : nat) : bool :=
+  if (in_dec Nat.eq_dec x l) then true else false.
+
+Fixpoint remove_one {A} (eq_dec : (forall x y : A, {x = y}+{x <> y})) (x : A) (l : list A) : list A := 
   match l with
-  | [] => false
-  | x'::xs => orb (eqb_zx_node x x') (inb_zx_node_list xs x) 
+      | [] => []
+      | x'::xs => if (eq_dec x x') then xs else x'::(remove_one eq_dec x xs)
   end.
 
-Definition zx_node_list_to_ids (l : list zx_node) : list nat :=
-  map (fun n => id_no n) l.
+Fixpoint largest_subset_and_rest_pool (lsplit lpool : list nat) : list nat * list nat  :=
+  match lsplit with
+  | [] => ([], lpool)
+  | x::xs =>  if (inb_zx_node_list lpool x) then 
+                match (largest_subset_and_rest_pool xs (remove_one Nat.eq_dec x lpool)) with
+                | (l1, l2) => (x :: l1, l2)
+                end
+              else
+                match (largest_subset_and_rest_pool xs lpool) with
+                | (l1, l2) => (l1, l2)
+                end
+  end.
 
-Definition get_connections (G : zx_graph) (node : zx_node) : list (zx_node * zx_node) :=
-  filter (fun n => orb (eqb_zx_node (fst n) node) (eqb_zx_node (snd n) node)) (edges G).
+Fixpoint largest_subset_and_rest_split (lsplit lpool : list nat) : list nat * list nat  :=
+  match lsplit with
+  | [] => ([], [])
+  | x::xs =>  if (inb_zx_node_list lpool x) then 
+                match (largest_subset_and_rest_split xs (remove_one Nat.eq_dec x lpool)) with
+                | (l1, l2) => (x :: l1, l2)
+                end
+              else
+                match (largest_subset_and_rest_split xs lpool) with
+                | (l1, l2) => (l1, x::l2)
+                end
+  end.
 
-Definition get_neighbors (G : zx_graph) (node : zx_node) : list zx_node :=
-  map (fun n => if (eqb_zx_node (fst n) node) then (snd n) else fst n) (get_connections G node).
+(* Test more? *)
+(* Compute (largest_subset_and_rest_split [1%nat; 2%nat; 3%nat; 4%nat; 4%nat] [4%nat; 5%nat; 4%nat; 3%nat]). *)
 
-Definition distribute_inputs_outputs (G : zx_graph) (cur_state : list zx_node) (cur_node : zx_node) : list zx_node * list zx_node :=
-  partition (fun n => (inb_zx_node_list cur_state n)) (get_neighbors G cur_node).
+(* Definition zx_node_list_to_ids (l : list zx_node) : list nat :=
+  map (fun n => id_no n) l. *)
 
-Definition get_cur_inputs (G : zx_graph) (cur_state : list zx_node) (cur_node : zx_node) : list zx_node :=
+
+Definition get_connections (G : zx_graph) (node : nat) : list (nat * nat) :=
+  filter (fun n => orb (node =? (fst n)) (node =? (snd n))) (edges G).
+
+Definition get_neighbors (G : zx_graph) (node : nat) : list nat :=
+  map (fun n => if ((fst n) =? node) then (snd n) else fst n) (get_connections G node).
+
+(* Check on pair order here *)
+Definition distribute_inputs_outputs (G : zx_graph) (cur_state : list nat) (cur_node : nat) : list nat * list nat :=
+  largest_subset_and_rest_split (get_neighbors G cur_node) cur_state.
+  
+Definition get_cur_inputs (G : zx_graph) (cur_state : list nat) (cur_node : nat) : list nat :=
   fst (distribute_inputs_outputs G cur_state cur_node).
 
-Definition get_cur_outputs (G : zx_graph) (cur_state : list zx_node) (cur_node : zx_node) : list zx_node :=
+Definition get_cur_outputs (G : zx_graph) (cur_state : list nat) (cur_node : nat) : list nat :=
   snd (distribute_inputs_outputs G cur_state cur_node).
 
-Definition split_cur_state (G : zx_graph) (cur_state : list zx_node) (cur_node : zx_node) : list zx_node * list zx_node :=
-  partition (fun n => (inb_zx_node_list (get_cur_inputs G cur_state cur_node) n)) cur_state.
-
-Definition get_goal_ordering (G : zx_graph) (cur_state : list zx_node) (cur_node : zx_node) : list zx_node :=
+Definition split_cur_state (G : zx_graph) (cur_state : list nat) (cur_node : nat) : list nat * list nat :=
+  largest_subset_and_rest_split cur_state (get_cur_inputs G cur_state cur_node).
+  
+Definition get_goal_ordering (G : zx_graph) (cur_state : list nat) (cur_node : nat) : list nat :=
   fst (split_cur_state G cur_state cur_node) ++ snd (split_cur_state G cur_state cur_node). 
 
-Definition get_cur_inputs_in_state (G : zx_graph) (cur_state : list zx_node) (cur_node : zx_node) : list zx_node :=
+Definition get_cur_inputs_in_state (G : zx_graph) (cur_state : list nat) (cur_node : nat) : list nat :=
   fst (split_cur_state G cur_state cur_node).
 
-Definition get_rest_cur_state (G : zx_graph) (cur_state : list zx_node) (cur_node : zx_node) : list zx_node :=
+Definition get_rest_cur_state (G : zx_graph) (cur_state : list nat) (cur_node : nat) : list nat :=
   snd (split_cur_state G cur_state cur_node).
 
-Definition get_new_state (G : zx_graph) (cur_state : list zx_node) (cur_node : zx_node) : list zx_node :=
+Definition get_new_state (G : zx_graph) (cur_state : list nat) (cur_node : nat) : list nat :=
   (repeat cur_node (length (get_cur_outputs G cur_state cur_node))) ++ 
   (get_rest_cur_state G cur_state cur_node).
 
-(* Rename these chief *)
-Lemma build_swap_structure_aux : forall l, length l = length (zx_node_list_to_ids l).
+(* Lemma build_swap_structure_aux : forall l, length l = length (zx_node_list_to_ids l).
 Proof.
   intros; unfold zx_node_list_to_ids; apply eq_sym; apply map_length.
-Qed.
+Qed. *)
+
+Lemma largest_subset_and_rest_split_length : 
+  forall lsplit lpool l1 l2,
+  largest_subset_and_rest_split lsplit lpool = (l1, l2) ->
+  length lsplit = ((length l1) + (length l2))%nat.
+Proof.
+  intros l1; induction l1.
+  - easy.
 
 (* Need to remove rewrites? *)
-Lemma build_node_structure_aux : forall G (cur_state : list zx_node) cur_node, 
+Lemma build_node_structure_aux : forall G (cur_state : list nat) cur_node, 
   length cur_state = ((length (get_cur_inputs_in_state G cur_state cur_node)) + (length (get_rest_cur_state G cur_state cur_node)))%nat.
 Proof.
   intros; unfold get_rest_cur_state, get_cur_inputs_in_state, split_cur_state.
   remember ((fun n : zx_node => inb_zx_node_list (get_cur_inputs G cur_state cur_node) n)) as f.
-  apply partition_length with (f := f). destruct (partition f cur_state); easy.
+  apply  with (f := f). destruct (partition f cur_state); easy.
 Qed.
 
 (* Need to remove rewrites? *)
-(* Lemma build_swap_structure_aux_aux : forall G (cur_state : list zx_node) cur_node, length cur_state = length (zx_node_list_to_ids (get_goal_ordering G cur_state cur_node)).
+(* Lemma build_swap_structure_aux_aux : forall G (cur_state : list nat) cur_node, length cur_state = length (zx_node_list_to_ids (get_goal_ordering G cur_state cur_node)).
 Proof.
   intros; unfold zx_node_list_to_ids; apply eq_sym; eapply eq_trans.
   eapply map_length. 
@@ -315,22 +366,18 @@ Proof.
 Qed. *)
 
 (* Check that this swap is correct *)
-Definition build_swap_structure (G : zx_graph) (cur_state : list zx_node) (cur_node : zx_node) : ZX (length cur_state) (length cur_state).
-Proof.
-  eapply cast.
-  - exact (build_swap_structure_aux cur_state).
-  - exact (build_swap_structure_aux cur_state).
-  - exact (create_arbitrary_swap (zx_node_list_to_ids cur_state) (zx_node_list_to_ids (get_goal_ordering G cur_state cur_node))).
-Defined.
+Definition build_swap_structure (G : zx_graph) (cur_state : list nat) (cur_node : nat) : ZX (length cur_state) (length cur_state) :=
+  create_arbitrary_swap cur_state (get_goal_ordering G cur_state cur_node).
 
 (* Need to consider box edges? *)
-Definition zx_node_to_spider (node : zx_node) (n m : nat) : ZX n m :=
-  match color node with 
-  | X_typ => X_Spider n m (angle node)
-  | _ => Z_Spider n m (angle node)
-  end.
+Definition zx_node_id_to_spider (G : zx_graph) (id_no n m : nat) : ZX n m :=
+  let node := (get_zx_node_by_id G id_no) in 
+    match color node with 
+    | X_typ => X_Spider n m (angle node)
+    | _ => Z_Spider n m (angle node)
+    end.
 
-Definition build_node_structure (G : zx_graph) (cur_state : list zx_node) (cur_node : zx_node) : 
+Definition build_node_structure (G : zx_graph) (cur_state : list nat) (cur_node : nat) : 
   ZX (length cur_state) ((length (get_cur_outputs G cur_state cur_node)) + (length (get_rest_cur_state G cur_state cur_node))).
 Proof.
   intros; eapply cast.
@@ -338,25 +385,27 @@ Proof.
   - reflexivity.
   - exact (pad_bot 
     (length (get_rest_cur_state G cur_state cur_node))
-    (zx_node_to_spider cur_node 
+    (zx_node_id_to_spider G cur_node 
       (length (get_cur_inputs_in_state G cur_state cur_node))
       (length (get_cur_outputs G cur_state cur_node)))).
 Defined.
 
-Definition one_node_translate (G : zx_graph) (cur_state : list zx_node) (cur_node : zx_node) : 
+Definition one_node_translate (G : zx_graph) (cur_state : list nat) (cur_node : nat) : 
   ZX (length cur_state) ((length (get_cur_outputs G cur_state cur_node)) + (length (get_rest_cur_state G cur_state cur_node))) :=
   (build_swap_structure G cur_state cur_node) ⟷ (build_node_structure G cur_state cur_node). 
 
-Definition gtb_last_fence_post (cur_state : list zx_node) (outputs : list zx_node) : ZX (length cur_state) (length outputs).
+Definition dummy_spider (n m : nat) : ZX n m := X_Spider n m R0.
+
+Definition gtb_last_fence_post (cur_state : list nat) (outputs : list nat) : ZX (length cur_state) (length outputs).
 Proof.
-  intros; destruct (eq_nat_decide (length outputs) (length (zx_node_list_to_ids cur_state))).
+  intros; destruct (eq_nat_decide (length outputs) (length cur_state)).
   - eapply cast.
-    + exact (build_swap_structure_aux cur_state). 
+    + reflexivity.
   (* There may be a better way to do this next line, necessary to prove equality like this? *)
     + eapply eq_nat_eq; exact e.
-    + exact (create_arbitrary_swap (zx_node_list_to_ids cur_state) (zx_node_list_to_ids outputs)).
+    + exact (create_arbitrary_swap cur_state outputs).
   (* Dummy value if output len not equal *)
-  - exact (X_Spider (length cur_state) (length outputs) R0).
+  - exact (dummy_spider (length cur_state) (length outputs)).
 Defined.
 
 (* Remove rewrites? *)
@@ -367,7 +416,7 @@ Proof.
   rewrite app_length; rewrite repeat_length; easy.
 Qed.
 
-Fixpoint graph_to_block_structure_aux (G : zx_graph) (node_order : list zx_node) (cur_state : list zx_node) : 
+Fixpoint graph_to_block_structure_aux (G : zx_graph) (node_order : list nat) (cur_state : list nat) : 
   ZX (length cur_state) (length (outputs G)).
 Proof.
   destruct node_order as [ | cur_node ns] eqn:E.
@@ -383,3 +432,9 @@ Defined.
 (* Translation function *)
 Definition graph_to_block_structure (G : zx_graph) : ZX (length (inputs G)) (length (outputs G)) :=
   graph_to_block_structure_aux G (nodes G) (inputs G).
+
+Definition node1 := mk_node 1%nat X_typ R1.
+Definition node2:= mk_node 2%nat Z_typ R0.
+
+(* Definition test1 := mk_graph
+  [] *)
